{
 "cells": [
  {
   "cell_type": "markdown",
   "metadata": {},
   "source": [
    "*Laurenz Mesiah A. Palanas* \n",
    "\n",
    "BSCS - BS Computer Science\n",
    "\n",
    "Student #21101123"
   ]
  },
  {
   "cell_type": "markdown",
   "metadata": {
    "vscode": {
     "languageId": "plaintext"
    }
   },
   "source": [
    "$\\textbf{Assignment}$\n",
    "Instructions:\n",
    "- Use latex.\n",
    "- Write your latex in jupyter notebook.\n",
    "- Push your answer to your github account.\n",
    "- Deadline is 2 weeks before finals.\n",
    "- Fail to submit 2 weeks before finals is an automatic 5.0 for this assignment.\n",
    "- Each problem is 25 points.\n",
    "\n",
    "1. Recall the definition of a rational number, denoted as $\\mathbb{Q}$. Prove that the Euler's number $e = \\Sigma_{k=0}^\\infty \\frac{1}{k!} \\notin \\mathbb{Q}$. A factorial is defined as $k! = (k)(k-1)(k-2)(k-3)..., \\forall k \\in \\mathbb{Z}^+$, note that $0! = 1$. Furthermore, a sum notation $\\Sigma_{k=0}^\\infty k = 0+ 1 + 2 + 3 +....+...$\n",
    "\n",
    "2. Prove Minkowski's Inequality for sums, $\\forall \\ p>1, (a_k, b_k)>0$:\n",
    "\\begin{gather}\n",
    "\\begin{bmatrix}\n",
    "\\Sigma_{k=1}^n |a_k + b_k|^p\n",
    "\\end{bmatrix}^\\frac{1}{p}\n",
    "\\leq\n",
    "\\begin{bmatrix}\n",
    "\\Sigma_{k=1}^n |a_k|^p\n",
    "\\end{bmatrix}^\\frac{1}{p}\n",
    "+\n",
    "\\begin{bmatrix}\n",
    "\\Sigma_{k=1}^n |b_k|^p\n",
    "\\end{bmatrix}^\\frac{1}{p}\n",
    "\\end{gather}\n",
    "\n",
    "3. Prove the triangle inequality $|x+y| \\leq |x| + |y|, \\forall (x,y) \\in \\mathbb{R}$\n",
    "\n",
    "4. Prove Sedrakayan's Lemma $\\forall u_i, v_i \\in \\mathbb{R}^+$:\n",
    "\\begin{gather}\n",
    "\\frac{(\\Sigma_{i=1}^n u_i)^2}{\\Sigma_{i=1}^n v_i}\n",
    "\\leq\n",
    "\\Sigma_{i=1}^n \\frac{(u_i)^2}{v_i}\n",
    "\\end{gather}\n",
    "\n",
    "1 Consider the functions $f(x) = 2x+1$, $g(x)=2y-1$, $j(x) = |f(x)+g(x)|$, and $h(x) = j(x)^2$, show for the following inequality that:\n",
    "\n",
    "\\begin{gather}\n",
    "\\sqrt{|f(x)|^2} \\geq \\sqrt{h(x)} - \\sqrt{|g(x)|^2}, \\forall (x,y) \\in \\mathbb{Z}^+\n",
    "\\end{gather}\n",
    "\n",
    "2. Prove Sedrakayan's Lemma if $u_i, v_i$ are square roots of an even integers:\n",
    "\\begin{gather}\n",
    "\\frac{(\\Sigma_{i=1}^n u_i)^2}{\\Sigma_{i=1}^n v_i}\n",
    "\\leq\n",
    "\\Sigma_{i=1}^n \\frac{(u_i)^2}{v_i}\n",
    "\\end{gather}"
   ]
  },
  {
   "cell_type": "markdown",
   "metadata": {
    "vscode": {
     "languageId": "plaintext"
    }
   },
   "source": [
    "$\\textbf{Answers}$ palanas\n",
    "\n",
    "$\\textbf{Solution Number 1}$\n",
    "\n",
    "1.) Recall the definition of a rational number, denoted as $\\mathbb{Q}$. Prove that the Euler's number $e = \\Sigma_{k=0}^\\infty \\frac{1}{k!} \\notin \\mathbb{Q}$. A factorial is defined as $k! = (k)(k-1)(k-2)(k-3)..., \\forall k \\in \\mathbb{Z}^+$, note that $0! = 1$. Furthermore, a sum notation $\\Sigma_{k=0}^\\infty k = 0+ 1 + 2 + 3 +....+...$\n",
    "\n",
    "\n",
    "Assume e = $\\mathbb{Q}$ , $e = \\frac{a}{b}$ where $a,b\\in \\mathbb\\Z\\ $ with no common factors (other than 1) and $b \\neq 0$\n",
    "\n",
    "\\begin{gather}\n",
    "e = \\sum_{k=0}^\\infty \\frac{1}{k} = 1 + \\frac{1}{1!} + \\frac{1}{2!} + \\frac{1}{3!} + \\frac{1}{4!} + ...\n",
    "\\end{gather}\n",
    "\n",
    "Multiply both sides factorial of $b!$\n",
    "\n",
    "\\begin{gather}\n",
    "b!e = b! (1 + \\frac{1}{1!} + \\frac{1}{2!} + \\frac{1}{3!} + \\frac{1}{4!} + \\frac{1}{5!} + ...)\n",
    "\\end{gather}\n",
    "\n",
    "\n",
    "as $k \\geq b$; each term in series $e$ has factor of $b!$ in the denominator\n",
    "\n",
    "\\begin{gather}\n",
    "\\frac{1}{k!} = \\frac{1}{k * (k-1)(k-2)(b*1)} * \\frac{1}{(b(b-1)(b-2)(2*1))} = \\frac{1}{(b-1)(b-2)...k}\n",
    "\\end{gather}\n",
    "\n",
    "substitute\n",
    "\n",
    "\\begin{gather}\n",
    "b!e = b!(1 + \\frac{1}{1!} + \\frac{1}{2!} + ... + \\frac{1}{(b+1)!} + \\frac{1}{(b+2)!} + ...)\n",
    "\\end{gather}\n",
    "\n",
    "\n",
    "$\\frac{1}{(b+1)!} + \\frac{1}{(b+2)!}$ are fractions with denominators that are $\\ge$ b.\n",
    "\n",
    "\n",
    "$\\therefore, \\forall$ the terms are $\\mathbb{Z}$ since $b!e$ is sum of $b!\\in\\mathbb{Z}$ and series of the $mathbb{Z}$. and e = $\\mathbb{Q}$, b!e is also $\\mathbb{Q}$.\n",
    "\n",
    "However, $b!e$ is the sum of $b!\\in\\mathbb{Z}$ and series of $\\mathbb{Z}$. and the sum of $\\mathbb{Z}$ is still equal to $\\mathbb{Z}$. This **leads to contradiction** as $b!e$ = $\\mathbb{Q}$ but must be $\\mathbb{Z}$.\n",
    "\n",
    "$\\therefore,$ **$e = \\sum_{k=0}^\\infty \\frac{1}{k!}\\notin\\mathbb{Q}$**\n",
    "\n",
    "\n",
    "\n"
   ]
  },
  {
   "cell_type": "markdown",
   "metadata": {},
   "source": [
    "$\\textbf{Solution Number 2}$\n",
    "\n",
    "2. Prove Minkowski's Inequality for sums, $\\forall \\ p>1, (a_k, b_k)>0$:\n",
    "\n",
    "\\begin{gather}\n",
    "\\left( \\sum_{k=1}^n |a_k + b_k|^p \\right)^{\\frac{1}{p}} \\leq \\left( \\sum_{k=1}^n |a_k|^p \\right)^{\\frac{1}{p}} + \\left( \\sum_{k=1}^n |b_k|^p \\right)^{\\frac{1}{p}}\n",
    "\\end{gather}\n",
    "\n",
    "\n",
    "Let's set $x_k = |a_k|^{\\frac{p}{p-1}}$ and $y_k = |b_k|^{\\frac{p}{p-1}}$. This implies that $\\frac{1}{p} + \\frac{1}{q} = 1$, where $q$ is the conjugate exponent of $p$. So, $q = \\frac{p}{p-1}$.\n",
    "\n",
    "Apply Hölder's inequality:\n",
    "\n",
    "\n",
    "\\begin{gather}\n",
    "\\sum_{k=1}^n |x_k y_k| \\leq \\left( \\sum_{k=1}^n |x_k|^p \\right)^{1/p} \\left( \\sum_{k=1}^n |y_k|^q \\right)^{1/q} \n",
    "\\end{gather}\n",
    "\n",
    "where $q$ is the conjugate exponent of $p$ given by $\\frac{1}{p} + \\frac{1}{q} = 1$.\n",
    "\n",
    "Let $x_k = \\frac{|a_k|}{\\left(\\sum_{k=1}^n |a_k|^p \\right)^{1/p}}$ and  $y_k = \\frac{|b_k|}{\\left(\\sum_{k=1}^n |b_k|^p \\right)^{1/p}}$\n",
    "\n",
    "Then, $\\sum_{k=1}^n |x_k|^p = 1$ and $\\sum_{k=1}^n |y_k|^q = 1.$\n",
    "\n",
    "\n",
    "Apply Hölder's inequality:\n",
    "\n",
    "\\begin{aligned}\n",
    "\\sum_{k=1}^n \\left| \\frac{a_k}{\\left(\\sum_{k=1}^n |a_k|^p \\right)^{1/p}} + \\frac{b_k}{\\left(\\sum_{k=1}^n |b_k|^p \\right)^{1/p}} \\right|^p &\\leq \\left( \\sum_{k=1}^n |x_k|^p \\right)^{1/p} \\left( \\sum_{k=1}^n |y_k|^q \\right)^{1/q} \\\\\n",
    "\\left( \\sum_{k=1}^n |a_k + b_k|^p \\right)^{1/p} &\\leq \\left( \\sum_{k=1}^n |a_k|^p \\right)^{1/p} \\left( \\sum_{k=1}^n |b_k|^p \\right)^{1/q}\n",
    "\\end{aligned} \\\\\n",
    "\n",
    "Since $\\frac{1}{p} + \\frac{1}{q} = 1,$ we have $q = \\frac{p}{p-1}$\n",
    "\n",
    "Hence, \n",
    "\n",
    "\\begin{aligned}\n",
    "\\left( \\sum_{k=1}^n |a_k + b_k|^p \\right)^{1/p} &\\leq \\left( \\sum_{k=1}^n |a_k|^p \\right)^{1/p} \\left( \\sum_{k=1}^n |b_k|^p \\right)^{1 - \\frac{1}{p}} \\\\\n",
    "&= \\left( \\sum_{k=1}^n |a_k|^p \\right)^{1/p} \\left( \\sum_{k=1}^n |b_k|^{\\frac{p}{p-1}} \\right)^{\\frac{1}{p-1}} \\\\\n",
    "&= \\left( \\sum_{k=1}^n |a_k|^p \\right)^{1/p} \\left( \\sum_{k=1}^n |b_k|^p \\right)^{\\frac{1}{p-1}}\n",
    "\\end{aligned} \n",
    "\n",
    "\n",
    "Minkowski's Inequality for sums is proven:\n",
    "\\begin{gather}\n",
    "\\left( \\sum_{k=1}^n |a_k + b_k|^p \\right)^{1/p} \\leq \\left( \\sum_{k=1}^n |a_k|^p \\right)^{1/p} + \\left( \\sum_{k=1}^n |b_k|^p \\right)^{1/p}\n",
    "\\end{gather}"
   ]
  },
  {
   "cell_type": "markdown",
   "metadata": {
    "vscode": {
     "languageId": "plaintext"
    }
   },
   "source": [
    "$\\textbf{Solution Number 3}$\n",
    "\n",
    "3. Prove the triangle inequality $|x+y| \\leq |x| + |y|, \\forall (x,y) \\in \\mathbb{R}$\n",
    "\n",
    "\n",
    "Case 1: $x \\geq 0 ; y \\geq 0$\n",
    "\n",
    "$|x+y| = x + y, |x| = x, and |y| = y$ \n",
    "\n",
    "$\\therefore,  x + y \\leq x + y$ Inequality holds for this case\n",
    "\n",
    "\n",
    "Case 2: $x \\geq 0 ; y < 0$\n",
    "\n",
    "$x - y \\leq x + y$ \n",
    "\n",
    "$-y \\leq x+y$\n",
    "\n",
    "$y \\geq 0$\n",
    "\n",
    "$\\therefore, Inequality holds for this case\n",
    "\n",
    "Case 3: $x < 0 ; y \\geq 0$\n",
    "\n",
    "$y-x \\leq x + y$ \n",
    "\n",
    "$-x \\leq x$\n",
    "\n",
    "$x \\geq 0$\n",
    "\n",
    "$\\therefore, Inequality holds for this case\n",
    "\n",
    "Case 4: $x < 0 ; y < 0$\n",
    "\n",
    "$-(x+y) \\leq x+y$ \n",
    "\n",
    "$x+y \\leq x+y$\n",
    "\n",
    "$\\therefore$, Inequality holds for this case\n",
    "\n",
    "\n",
    "$\\therefore,$ by examining all cases, it is shown that $|x+y| \\leq |x| + |y|, \\forall (x,y) \\in \\mathbb{R}$\n",
    "\n"
   ]
  },
  {
   "cell_type": "markdown",
   "metadata": {},
   "source": [
    "$\\textbf{Solution Number 4}$\n",
    "\n",
    "4.1 - Prove Sedrakayan's Lemma $\\forall u_i, v_i \\in \\mathbb{R}^+$:\n",
    "\\begin{gather}\n",
    "\\frac{(\\Sigma_{i=1}^n u_i)^2}{\\Sigma_{i=1}^n v_i}\n",
    "\\leq\n",
    "\\Sigma_{i=1}^n \\frac{(u_i)^2}{v_i}\n",
    "\\end{gather}\n",
    "\n",
    "4.2 - Consider the functions $f(x) = 2x+1$, $g(x)=2y-1$, $j(x) = |f(x)+g(x)|$, and $h(x) = j(x)^2$, show for the following inequality that:\n",
    "\n",
    "\\begin{gather}\n",
    "\\sqrt{|f(x)|^2} \\geq \\sqrt{h(x)} - \\sqrt{|g(x)|^2}, \\forall (x,y) \\in \\mathbb{Z}^+\n",
    "\\end{gather}\n",
    "\n",
    "4.3 - Prove Sedrakayan's Lemma if $u_i, v_i$ are square roots of an even integers:\n",
    "\\begin{gather}\n",
    "\\frac{(\\Sigma_{i=1}^n u_i)^2}{\\Sigma_{i=1}^n v_i}\n",
    "\\leq\n",
    "\\Sigma_{i=1}^n \\frac{(u_i)^2}{v_i}\n",
    "\\end{gather}"
   ]
  },
  {
   "cell_type": "markdown",
   "metadata": {},
   "source": [
    "**4.1**\n",
    "\n",
    "Prove Sedrakayan's Lemma $\\forall u_i, v_i \\in \\mathbb{R}^+$:\n",
    "\\begin{gather}\n",
    "\\frac{(\\Sigma_{i=1}^n u_i)^2}{\\Sigma_{i=1}^n v_i}\n",
    "\\leq\n",
    "\\Sigma_{i=1}^n \\frac{(u_i)^2}{v_i}\n",
    "\\end{gather}\n",
    "\n",
    "**Solution:**\n",
    "\n",
    "\n",
    "To prove Sedrakayan's Lemma, we'll use the Cauchy-Schwarz Inequality, which states that for any sequences of real numbers $a_i$ and $b_i$, the following holds:\n",
    "\n",
    "$\\sum_{i=1}^n a_i b_i)^2 \\leq (\\sum_{i=1}^n a_i^2)(\\sum_{i=1}^n b_i^2$\n",
    "\n",
    "\n",
    "\n",
    "Apply Cauchy-Schwarz Inequality to $\\sqrt{v_i}$ and $\\frac{u_i}{\\sqrt{v_i}}$:\n",
    "\n",
    "\\begin{gather}\n",
    "(\\sum_{i=1}^n \\sqrt{v_i} \\cdot \\frac{u_i}{\\sqrt{v_i}})^2 \\leq (\\sum_{i=1}^n (\\sqrt{v_i})^2)(\\sum_{i=1}^n (\\frac{u_i}{\\sqrt{v_i}})^2)\n",
    "\\end{gather}\n",
    "\n",
    "\n",
    "Simplify:\n",
    "\n",
    "\\begin{gather}\n",
    "(\\sum_{i=1}^n u_i)^2 \\leq (\\sum_{i=1}^n v_i)(\\sum_{i=1}^n \\frac{u_i^2}{v_i})\n",
    "\\end{gather}\n",
    "        \n",
    "\n",
    "Divide both sides by $\\sum_{i=1}^n v_i$:\n",
    "        \n",
    "\\begin{gather}\n",
    "\\frac{(\\sum_{i=1}^n u_i)^2}{\\sum_{i=1}^n v_i} \\leq \\sum_{i=1}^n \\frac{u_i^2}{v_i}\n",
    "\\end{gather}\n",
    "\n",
    "\n",
    "$\\therefore$, Sedrakayan's Lemma is proven.\n",
    "    \n"
   ]
  },
  {
   "cell_type": "markdown",
   "metadata": {},
   "source": [
    "    \n",
    "**4.2**\n",
    "\n",
    "Consider the functions $f(x) = 2x+1$, $g(x)=2y-1$, $j(x) = |f(x)+g(x)|$, and $h(x) = j(x)^2$, show for the following inequality that:\n",
    "\n",
    "\\begin{gather}\n",
    "\\sqrt{|f(x)|^2} \\geq \\sqrt{h(x)} - \\sqrt{|g(x)|^2}, \\forall (x,y) \\in \\mathbb{Z}^+\n",
    "\\end{gather}\n",
    "\n",
    "\n",
    "Solution:\n",
    "\n",
    "Since $h(x) = j(x)^2$ and $j(x) = |f(x) + g(x)| = |2x + 1 + 2y - 1| = |2x + 2y| = 2|x + y|$, we have:\n",
    "\n",
    "\\begin{gather}\n",
    "h(x) = (2|x + y|)^2 = 4(x + y)^2\n",
    "\\end{gather}    \n",
    "\n",
    "So, we need to show that $2y \\geq 2|x + y|$ holds for all $(x, y) \\in \\mathbb{Z}^+$.\n",
    "\n",
    "This inequality holds true because the absolute value function makes $|x + y|$ non-negative, and multiplying it by $2$ makes it less than or equal to $2y$."
   ]
  },
  {
   "cell_type": "markdown",
   "metadata": {},
   "source": [
    "**4.3**\n",
    "\n",
    "Prove Sedrakayan's Lemma if $u_i, v_i$ are square roots of an even integers:\n",
    "\\begin{gather}\n",
    "\\frac{(\\Sigma_{i=1}^n u_i)^2}{\\Sigma_{i=1}^n v_i}\n",
    "\\leq\n",
    "\\Sigma_{i=1}^n \\frac{(u_i)^2}{v_i}\n",
    "\\end{gather}\n",
    "\n",
    "**Solution**\n",
    "Given Sedrakayan's Lemma for square roots of even integers, we can utilize the fact that if $u_i, v_i$ are square roots of even integers, then $u_i^2, v_i$ are integers.\n",
    "        \n",
    "Since $u_i^2, v_i$ are integers, we can apply Sedrakayan's Lemma directly:\n",
    "        \n",
    "\\begin{gather}\n",
    "\\frac{(\\sum_{i=1}^n u_i^2)}{(\\sum_{i=1}^n v_i)} \\leq \\sum_{i=1}^n \\frac{u_i^2}{v_i}\n",
    "\\end{gather}\n",
    "        \n",
    "This proves Sedrakayan's Lemma for square roots of even integers."
   ]
  }
 ],
 "metadata": {
  "language_info": {
   "name": "python"
  }
 },
 "nbformat": 4,
 "nbformat_minor": 2
}
