{
 "cells": [
  {
   "cell_type": "markdown",
   "metadata": {},
   "source": [
    "**Laurenz Mesiah A. Palanas** \n",
    "\n",
    "**BSCS** - *BS Computer Science* 1\n",
    "\n",
    "21101123\n",
    "\n",
    "\n",
    "$\\textbf{Programming Assignments}$\n",
    "-\n",
    "\n",
    "Intructions:\n",
    "- Use Latex to write your solution.\n",
    "- Push your solution to your github repository.\n",
    "\n",
    "**Task 1:**\n",
    "Consider the following experiment:\n",
    "\n",
    "1. The experiment consists of $n$ identical trials.\n",
    "2. The outcome of each trial falls into one of $k$ classes or cells.\n",
    "3. The probability that the outcome of a single trial falls into cell $i$, is $p_i,i = 1,2,...,k$ and remains the same from trial to trial. Notice that $p_1+p_2+p_3+···+p_k =1.$\n",
    "4. The trials are independent.\n",
    "5. The random variables of interest are $Y_1 , Y_2 , . . . , Y_k$, where $Y_i$ equals the number of trials for which the outcome falls into cell $i$. Notice that $Y_1 +Y_2 +Y_3 +···+Y_k =n$.\n",
    "6. The joint probability distribution $P(y) = \\frac{n!}{y_1!y_2!y_3!...y_n!} P_1^{y_1} P_2^{y_2} P_3^{y_3}....P_n^{y_n}$\n",
    "\n",
    "Question 1: Show that the expected value $E[y] = \\Sigma y \\cdotp P(y) = n \\cdot p_i$\n",
    "\n",
    "Question 2: Given the following data\n",
    "\\begin{gather}\n",
    "\\begin{bmatrix}\n",
    "\\begin{array}{c|c}\n",
    "Age & Proportion \\\\\n",
    "18-24 & 0.18 \\\\\n",
    "25-34 & 0.23 \\\\\n",
    "35-44 & 0.16 \\\\\n",
    "45-64 & 0.27 \\\\\n",
    "65-100 & 0.16 \\\\\n",
    "\\end{array}\n",
    "\\end{bmatrix}\n",
    "\\end{gather}\n",
    "\n",
    "If 500 adults are sampled  randomly, find the probability rhat the sample contains 100 person between 18 and 24, 200 between the ages of 25 and 34, and 200 between the ages of 45 and 64.. What is the expected value for to obtain a person in the 65 and above?\n",
    "\n",
    "\n",
    "\n",
    "**Task 2:** Consider the following experiment:\n",
    "\n",
    "1. The experiment consists of a fixed number, $n$, of identical trials.\n",
    "2. Each trial results in one of two outcomes: success, $S$, or failure, $F$.\n",
    "3. The probability of success on a single trial is equal to some value $p$ and remains the same from trial to trial. The probability of a failure is equal to q = $(1 − p)$.\n",
    "4. The trials are independent.\n",
    "5. The random variable of interest is $Y$ , the number of successes observed during the $n$ trials.\n",
    "\n",
    "*Question 1:* From the following steps shown above, derive the probability distribution of the experiment.\n",
    "\n",
    "*Question 2:* Show that the expectation of this probability distribution is $E[y] = \\Sigma y \\cdotp P(y) = np$.\n",
    "\n",
    "*Question 3:* TExperience has shown that 30% of all persons afflicted by a certain illness recover. A drug company has developed a new medication. Ten people with the illness were selected at random and received the medication; nine recovered shortly thereafter. Suppose that the medication was absolutely worthless. What is the probability that at least nine of ten receiving the medication will recover?\n",
    "\n",
    "*Question 4:* Suppose that a lot of 5000 electrical fuses contains 5% defectives. If a sample of 5 fuses is tested, find the probability of observing at least one defective.\n",
    "\n",
    "\n",
    "**Task 3:** Consider a probility distribution of $p(y) = \\frac{\\lambda^y}{y!} e^{-\\lambda}$.\n",
    "\n",
    "*Question 1:* Find a general formula for the expected value of this distribution.\n",
    "\n",
    "*Question 2:* A certain type of tree has seedlings randomly dispersed in a large area, with the mean density of seedlings being approximately five per square yard. If a forester randomly locates ten 1-square-yard sampling regions in the area, find the probability that none of the regions will contain seedlings.\n"
   ]
  },
  {
   "cell_type": "markdown",
   "metadata": {},
   "source": [
    "**Task 1**\n",
    "\n",
    "Consider the following experiment:\n",
    "\n",
    "*We conduct $n$ identical trials.\n",
    "Each trial's outcome belongs to one of $k$ classes or cells.\n",
    "The probability of a single trial's outcome falling into cell $i$ is $p_i$, where $i = 1,2,...,k$, and the sum of all probabilities equals $1$.\n",
    "The trials are independent.\n",
    "We define random variables of interest $Y_1 , Y_2 , . . . , Y_k$, where $Y_i$ represents the number of trials with outcomes falling into cell $i$. Note that $Y_1 +Y_2 +Y_3 +···+Y_k =n$.\n",
    "The joint probability distribution $P(y) = \\frac{n!}{y_1!y_2!y_3!...y_n!} P_1^{y_1} P_2^{y_2} P_3^{y_3}....P_n^{y_n}$*\n",
    "\n",
    "$\\textbf{Question 1:}$ Demonstrate that the expected value $E[y] = \\Sigma y \\cdot P(y) = n \\cdot p_i$\n",
    "\n",
    "Step 1: Express the expected value $E[y]$ in terms of $P(y)$:\n",
    "\n",
    "\\begin{gather}\n",
    "E[y] = \\Sigma_{y} , y \\cdot P(y)\n",
    "\\end{gather}\n",
    "\n",
    "\n",
    "Step 2: Substitute the given joint probability distribution for $P(y)$.\n",
    "\n",
    "\\begin{gather}\n",
    "E[y] = \\Sigma_{y} , y \\cdot \\left(\\frac{n!}{y_1!y_2!y_3!...y_k!} \\cdot p_1^{y_1} p_2^{y_2} p_3^{y_3}....p_k^{y_k}\\right) \n",
    "\\end{gather}\n",
    "\n",
    "Step 3: Expand the sum:\n",
    "\n",
    "\\begin{gather}\n",
    "E[y] = \\Sigma_{y} \\frac{n!}{y_1!y_2!y_3!...y_k!} \\cdot (y_1 \\cdot p_1) \\cdot (y_2 \\cdot p_2) \\cdot (y_3 \\cdot p_3) \\ldots (y_k \\cdot p_k)\n",
    "\\end{gather}\n",
    "\n",
    "\n",
    "\n",
    "Step 4: Rearrange the terms:\n",
    "\n",
    "\\begin{gather}\n",
    "E[y] = \\frac{n!}{y_1!y_2!y_3!...y_k!} \\cdot \\Sigma_{y} (y_1 \\cdot p_1) \\cdot (y_2 \\cdot p_2) \\cdot (y_3 \\cdot p_3) \\ldots (y_k \\cdot p_k)\n",
    "\\end{gather}\n",
    "\n",
    "\n",
    "\n",
    "Step 5: Notice that the sum is a product of sums:\n",
    "\n",
    "\\begin{gather}\n",
    "E[y] = \\frac{n!}{y_1!y_2!y_3!...y_k!} \\cdot ( \\Sigma_{y_1} ,y_1 \\cdot p_1) \\cdot (\\Sigma_{y_2} , y_2 \\cdot p_2) \\cdot ( \\Sigma_{y_3} , y_3 \\cdot p_3) \\ldots ( \\Sigma_{y_k} , y_k \\cdot p_k)\n",
    "\\end{gather}\n",
    "\n",
    "\n",
    "Step 6: Each individual sum represents the expected value of a binomial distribution with parameters $n$ and $p_i$:\n",
    "\n",
    "\\begin{gather}\n",
    "E[Y_i] = n \\cdot p_i\n",
    "\\end{gather}\n",
    "\n",
    "\n",
    "\n",
    "Step 7: Substitute the expected values of each $Y_i$:\n",
    "\n",
    "\\begin{gather}\n",
    "E[y] = \\frac{n!}{y_1!y_2!y_3!...y_k!} \\cdot (n \\cdot p_1) \\cdot (n \\cdot p_2) \\cdot (n \\cdot p_3) \\ldots (n \\cdot p_k)\n",
    "\\end{gather}\n",
    "\n",
    "\n",
    "Step 8: Notice that $n!$ and $y_1!y_2!y_3!...y_k!$ cancel out:\n",
    "\n",
    "\\begin{gather}\n",
    "E[y] = n \\cdot p_1 \\cdot n \\cdot p_2 \\cdot n \\cdot p_3 \\ldots n \\cdot p_k\n",
    "\\end{gather}\n",
    "\n",
    "\n",
    "\n",
    "We simplify the expression by combining terms and recognizing that the coefficient $(y_1!y_2!y_3!...y_k!)$ can be simplified to $n!$, the number of permutations of outcomes.\n",
    "\n",
    "Step 9: Simplify:\n",
    "\n",
    "\\begin{gather}\n",
    "E[y] = n (p_1 \\cdot p_2 \\cdot p_3 \\ldots p_k)\n",
    "\\end{gather}\n",
    "\n",
    "\n",
    "Step 10: Recall that $p_1 + p_2 + p_3 + \\ldots + p_k = 1 $:\n",
    "\n",
    "\\begin{gather}\n",
    "E[y] = n \\cdot 1 \\\\\n",
    "E[y] = n \\cdot p_i\n",
    "\\end{gather}\n",
    "\n",
    "\n",
    "\n",
    "\n",
    "$\\therefore$ the expected value $E[y]$ = $\\Sigma y \\cdot P(y)$, which equals $n \\cdot p_i$.\n",
    "\n",
    "\n",
    "\n",
    "\n",
    "\n",
    "$\\textbf{Question 2:}$\n",
    "\n",
    "Given the following data\n",
    "\\begin{gather}\n",
    "\\begin{bmatrix}\n",
    "\\begin{array}{c|c}\n",
    "Age & Proportion \\\\\n",
    "18-24 & 0.18 \\\\\n",
    "25-34 & 0.23 \\\\\n",
    "35-44 & 0.16 \\\\\n",
    "45-64 & 0.27 \\\\\n",
    "65-100 & 0.16 \\\\\n",
    "\\end{array}\n",
    "\\end{bmatrix}\n",
    "\\end{gather}\n",
    "\n",
    "*If 500 adults are sampled  randomly, find the probability rhat the sample contains 100 person between 18 and 24, 200 between the ages of 25 and 34, and 200 between the ages of 45 and 64.. What is the expected value for to obtain a person in the 65 and above?*\n",
    "\n",
    "\n",
    "\n",
    "Given:\n",
    "\n",
    "$n = 500$ **(total number of sampled adults)**\n",
    "$p_{65-100} = 0.16$ **(probability of selecting a person aged 65 and above)**\n",
    "\n",
    "Step 1: Apply the Formula\n",
    "\n",
    "The expected value $E[Y_{65+}]$ is calculated as:\n",
    "\n",
    "$ E[Y_{65+}] = n \\cdot p_{65-100}$\n",
    "\n",
    "\n",
    "Step 2: Substitute Values\n",
    "\n",
    "$ E[Y_{65+}] = 500 \\cdot 0.16$\n",
    "**$ E[Y_{65+}] = 80$**\n",
    "\n",
    "\n",
    "Hence, **the expected number of people aged between 65 to 100 is 80**."
   ]
  },
  {
   "cell_type": "markdown",
   "metadata": {},
   "source": [
    "**Task 2**\n",
    "\n",
    "$\\textbf{Question 1:}$\n",
    "\n",
    "*From the following steps shown above, derive the probability distribution of the experiment.*\n",
    "\n",
    "The probability distribution of $Y$ follows a binomial distribution, which is calculated using the binomial probability mass function:\n",
    "\n",
    "\\begin{gather}\n",
    "P(Y = y) = \\binom{n}{y} \\cdot p^y \\cdot q^{n-y}\n",
    "\\end{gather}\n",
    "\n",
    "$\\ni$:\n",
    "\n",
    "- $P(Y = y)$ represents the probability of observing $y$ successes in $n$ trials.\n",
    "- $\\binom{n}{y}$ denotes the binomial coefficient, representing the number of ways to choose $y$ successes out of $n$ trials.\n",
    "- $p^y$ represents the probability of having $y$ successes.\n",
    "- $q^{n-y}$ represents the probability of having $(n - y)$ failures.\n",
    "\n",
    "\n",
    "\n",
    "$\\textbf{Question 2:}$\n",
    "\n",
    "*Show that the expectation of this probability distribution is $E[y] = \\Sigma y \\cdotp P(y) = np$.*\n",
    "\n",
    "Step 1: Define the Expectation\n",
    "\n",
    "\\begin{gather}\n",
    "E[y] = \\Sigma_{y = 0}^n \\cdot P(y).\n",
    "\\end{gather}\n",
    "\n",
    "\n",
    "Step 2: Substitute the Binomial Probability Mass Function\n",
    "\n",
    "\\begin{gather}\n",
    "E[y] = \\Sigma_{y = 0}^n \\cdot \\binom{n}{y} \\cdot p^y \\cdot q^{n-y}.\n",
    "\\end{gather}\n",
    "\n",
    "\n",
    "Step 3: Simplify the Expression\n",
    "\n",
    "Substitute $q$ with $1-p$ and rearrange terms.\n",
    "\n",
    "\\begin{gather}\n",
    "E[y] = \\Sigma_{y = 0}^n \\cdot \\frac{n!}{y!(n-y)!} \\cdot (p)^y \\cdot (1-p)^{(n-y)}.\n",
    "\\end{gather}\n",
    "\n",
    "\n",
    "Step 4: Factor Out Constants\n",
    "\n",
    "Since $p$ is constant, it can be factored out of the summation.\n",
    "\n",
    "\\begin{gather}\n",
    "E[y] = np \\cdot \\Sigma_{y = 0}^n \\cdot \\frac{(n-1)!}{(y-1)!(n-y)!} \\cdot (p)^{(y-1)} \\cdot (1-p)^{(n-y)}.\n",
    "\\end{gather}\n",
    "\n",
    "\n",
    "Step 5: Rearrange the Terms\n",
    "\n",
    "\\begin{gather}\n",
    "E[y] = np \\cdot \\Sigma_{y = 1}^n \\cdot \\frac{(n-1)!}{(y-1)!(n-y)!} \\cdot (p)^{(y-1)} \\cdot (1-p)^{(n-y)}.\n",
    "\\end{gather}\n",
    "\n",
    "\n",
    "Step 6: Apply the Binomial Theorem\n",
    "\n",
    "Use the binomial theorem to expand $(p + q)^ {n -1}$.\n",
    "\n",
    "\\begin{gather}\n",
    "(p + q)^ {n-1} = \\Sigma_{k = 0}^{n-1} \\binom{n-1}{y} \\cdot (p)^{(k)} \\cdot (q)^{(n-1-k)}\n",
    "\\end{gather}\n",
    "\n",
    "\n",
    "By comparing terms to the binomial theorem, we find:\n",
    "\n",
    "\\begin{gather}\n",
    "(p + q)^ {n-1} = \\Sigma_{y = 0}^{n} \\cdot \\frac{(n-1)!}{(y)!(n-y)!} \\cdot (p)^{(y)} \\cdot (q)^{(n-y)}\n",
    "\\end{gather}\n",
    "\n",
    "Step 7: Simplify the expression\n",
    "\n",
    "The expansion of $(p + (1-p))^{n-1}$ is $1^{n-1}$, which equals 1. Therefore, the sum becomes 1.\n",
    "\n",
    "This simplifies to:\n",
    "\n",
    "\n",
    "$E[y] = np \\cdot 1$, leading to the final simplification of $E[y] = np$.\n",
    "\n",
    "\n",
    "\n",
    "In conclusion, the expectation of a binomial distribution, $E[y] = np$, confirms that the mean equals the product of the number of trials and the probability of success.\n",
    "\n",
    "$\\textbf{Question 3:}$ *Probability of Recovery*\n",
    "\n",
    "*TExperience has shown that 30% of all persons afflicted by a certain illness recover. A drug company has developed a new medication. Ten people with the illness were selected at random and received the medication; nine recovered shortly thereafter. Suppose that the medication was absolutely worthless. What is the probability that at least nine of ten receiving the medication will recover?*\n",
    "\n",
    "Given:\n",
    "\n",
    "Probability of success (recovery) $p = 0.30$\n",
    "\n",
    "Number of trials $n = 10$\n",
    "\n",
    "Number of successes (recoveries) $y = 9$\n",
    "\n",
    "Using the binomial probability mass function:\n",
    "\n",
    "\n",
    "Solution:\n",
    "\n",
    "\n",
    "\\begin{gather}\n",
    "P(Y \\geq 9) = P(Y = 9) + P(Y = 10) \\\\\n",
    "P(Y \\geq 9) = \\binom{10}{9} \\cdot (0.30)^9 \\cdot (1 - 0.30)^{10-9} + \\binom{10}{10} \\cdot (1 - 0.30)^{10-10} \\\\\n",
    "P(Y \\geq 9) = 10 \\cdot (0.30)^9 \\cdot (0.70)^1 + 1 \\cdot (0.30)^{10} \\cdot (0.70)^0 \\\\\n",
    "P(Y \\geq 9) = 10 \\cdot (0.30)^9 \\cdot 0.70 + (0.30)^{10} \\\\\n",
    "P(Y \\geq 9) \\approx 0.000137781 + 0.0000059049 \\\\\n",
    "P(Y \\geq 9) \\approx 0.0001436869%\n",
    "\\end{gather}\n",
    "\n",
    "\n",
    "Thus, the probability of at least nine out of ten individuals recovering is **approximately $0.014%$.**\n",
    "\n",
    "\n",
    "$\\textbf{Question 4:}$ Probability of Observing at Least One Defective Fuse\n",
    "\n",
    "*Suppose that a lot of 5000 electrical fuses contains 5% defectives. If a sample of 5 fuses is tested, find the probability of observing at least one defective.*\n",
    "\n",
    "Given:\n",
    "\n",
    "Probability of success (a fuse being non-defective) $p = 0.95$\n",
    "\n",
    "Number of trials $n = 5$\n",
    "\n",
    "Solution:\n",
    "\n",
    "\\begin{gather}\n",
    "P(\\text{At least one defective}) = 1 - P(\\text{No defective}) \\\\\n",
    "P(\\text{At least one defective}) = 1 - P(Y = 0)\n",
    "\\end{gather}\n",
    "\n",
    "\n",
    "\n",
    "Using the binomial probability mass function:\n",
    "\n",
    "\\begin{gather}\n",
    "P(Y=0) = \\binom {5}{0} \\cdot (0.05)^0 \\cdot (1 - 0.05)^{5-0} \\\\\n",
    "P(Y = 0) = (0.95)^5 \\\\\n",
    "P(\\text{At least one defective}) = 1 - (0.95)^5 \\\\\n",
    "P(\\text{At least one defective}) \\approx 1 - 0.7738 \\\\\n",
    "P(\\text{At least one defective}) \\approx 0.2262 \\\\\n",
    "\\end{gather}\n",
    "\n",
    "\n",
    "\n",
    "$\\therefore$ the probability of observing at least one defective fuse in a sample of 5 fuses is approximately $0.2262$ or $22.62%$."
   ]
  },
  {
   "cell_type": "markdown",
   "metadata": {},
   "source": [
    "**Task 3:** Consider a probility distribution of $p(y) = \\frac{\\lambda^y}{y!} e^{-\\lambda}$.\n",
    "\n",
    "$\\textbf{Question 1:}$ \n",
    "\n",
    "Find a general formula for the expected value of this distribution.\n",
    "\n",
    "\n",
    "Given probability distribution: \n",
    "\n",
    "\n",
    "\\begin{gather}\n",
    "P(\\text{At least one defective}) = 1 - P(\\text{No defective}) \\\\\n",
    "P(\\text{At least one defective}) = 1 - P(Y = 0)\n",
    "\\end{gather}\n",
    "p(y) = \\frac{\\lambda^y}{y!} e^{-\\lambda}\n",
    "\n",
    "Expected value formula: \n",
    "\n",
    "\\begin{gather}\n",
    "E[Y] = \\Sigma_{y=0} ^ \\infty \\, y \\cdot p(y)\n",
    "\\end{gather}\n",
    "\n",
    "\n",
    "\n",
    "Substitute the Probability Distribution into the Expected Value Formula\n",
    "\n",
    "\\begin{gather}\n",
    "E[Y] = \\Sigma_{y=0} ^ \\infty \\, y \\cdot \\frac{\\lambda^y}{y!} e^{-\\lambda}\n",
    "\\end{gather}\n",
    "\n",
    "\n",
    "Factor out Constants\n",
    "\n",
    "\\begin{gather}\n",
    "E[Y] = e^{-\\lambda} \\Sigma_{y=0} ^ \\infty \\, \\frac{\\lambda^y}{(y - 1)!} \n",
    "\\end{gather}\n",
    "\n",
    "\n",
    "\n",
    "Since $y = 0$ makes $\\frac{\\lambda^y}{(y - 1)!}$ undefined, we shift the index of summation to start from $y = 1$.\n",
    "\n",
    "\\begin{gather}\n",
    "E[Y] = e^{-\\lambda} \\Sigma_{y=1} ^ \\infty \\, \\frac{\\lambda^y}{(y - 1)!} \n",
    "\\end{gather}\n",
    "\n",
    "\n",
    "Rewrite $\\frac{\\lambda^y}{(y - 1)!}$ as $\\frac{\\lambda^{(y-1)+ 1}}{(y - 1)!}$\n",
    "\n",
    "\\begin{gather}\n",
    "E[Y] = e^{-\\lambda} \\Sigma_{y=1} ^ \\infty \\,  \\frac{\\lambda^{(y-1)+ 1}}{(y - 1)!}\n",
    "\\end{gather}\n",
    "\n",
    "\n",
    "Change the index of summation to start from $y = 0$ to simplify the expression.\n",
    "\n",
    "\\begin{gather}\n",
    "E[Y] = e^{-\\lambda} \\Sigma_{y=0} ^ \\infty \\,  \\frac{\\lambda^{y+1}}{y!}\n",
    "\\end{gather}\n",
    "\n",
    "\n",
    "Factor out $\\lambda$\n",
    "\n",
    "\\begin{gather}\n",
    "E[Y] = e^{-\\lambda} \\lambda \\Sigma_{y=0} ^ \\infty \\, \\frac {\\lambda^{y}}{y!}\n",
    "\\end{gather}\n",
    "\n",
    "\n",
    "Recall that $e^{\\lambda} =  \\Sigma_{y=0} ^ \\infty \\, \\frac {\\lambda^{y}}{y!}$\n",
    "\n",
    "\\begin{gather}\n",
    "E[Y] = e^{-\\lambda} \\lambda e^{\\lambda} \n",
    "\\end{gather}\n",
    "\n",
    "\n",
    "Simplify: \n",
    "\\begin{gather}\n",
    "E[Y] =  \\lambda\n",
    "\\end{gather}\n",
    "\n",
    "\n",
    "$\\therefore$, the expected value of the given distribution is **$E[Y] =  \\lambda$**\n",
    "\n",
    "\n",
    "\n",
    "$\\textbf{Question 2:}$ \n",
    "\n",
    "A certain type of tree has seedlings randomly dispersed in a large area, with the mean density of seedlings being approximately five per square yard. If a forester randomly locates ten 1-square-yard sampling regions in the area, find the probability that none of the regions will contain seedlings.\n",
    "\n",
    "Given:\n",
    "- $\\lambda = 5$\n",
    "\n",
    "Solution: \n",
    "\n",
    "Use the formula for the Poisson distribution:\n",
    "\n",
    "\\begin{gather}\n",
    "P(Y = y) = \\frac{\\lambda^y}{y!} e^{-\\lambda}\n",
    "\\end{gather}\n",
    "\n",
    "\n",
    "For $y = 0$:\n",
    "\n",
    "\\begin{gather}\n",
    "P(Y = 0) = \\frac{5^0}{0!} e^{-5} \\\\\n",
    "= e^{-5} \n",
    "\\end{gather}\n",
    "\n",
    "\n",
    "Calculating probability:\n",
    "\n",
    "\\begin{gather}\n",
    "P(Y = 0) \\approx e^{-5}  \\\\\n",
    "\\approx 0.006737947\n",
    "\\end{gather}\n",
    "\n",
    "\n",
    "$\\therefore$ the probability is approximately $ 0.0067$ or $ 0.67\\%$ that none of the regions will contain seedlings."
   ]
  }
 ],
 "metadata": {
  "language_info": {
   "name": "python"
  }
 },
 "nbformat": 4,
 "nbformat_minor": 2
}
